demo/DemoBspec.v
@@ -12,8 +12,6 @@ Require Import SymbolTable DemoB.
   The specification of DemoB.prog in lts li_C -> li_C
  *)
 
-Definition skel0 := erase_program DemoB.prog.
-
 Inductive state: Type :=
 | Callstate
     (i: int)
@@ -25,12 +23,7 @@ Inductive state: Type :=
     (s: int)
     (m: mem).
 
-Definition get_mem (st: state): mem :=
-  match st with
-  | Callstate _ m => m
-  | Interstate _ m => m
-  | Returnstate _ m => m
-  end.
+Definition genv := Genv.t fundef unit.
 
 Section WITH_SE.
   Context (se: Genv.symtbl).
@@ -84,8 +77,61 @@ Inductive final_state: state -> reply li_c  -> Prop :=
       s m :
       final_state (Returnstate s m) (cr (Vint s) m).
 
-(* no actual program context, donot need to check available internal function implementation*)
-Definition valid_query (q : query li_c): bool := true.
+End WITH_SE.
+(*
+Section WITH_SE.
+  Context (ge: genv).
+
+Inductive initial_state : query li_c -> state -> Prop :=
+| initial_state_intro
+    args m i gb
+    (SYMB: Genv.symbol_address ge g_id Ptrofs.zero = Vptr gb Ptrofs.zero)
+(*    (RANGE: 0 <= i.(Int.intval) < MAX) *)
+    (VS: args = (Vint i:: nil)):
+    initial_state (cq (Vptr gb Ptrofs.zero) int_int_sg ((Vint i) :: nil) m) (Callstate i m).
+
+Inductive at_external: state -> query li_c -> Prop :=
+| at_external_intro
+    fb i m
+    (FINDG: Genv.symbol_address ge f_id Ptrofs.zero = Vptr fb Ptrofs.zero):
+    at_external (Interstate i m) (cq (Vptr fb Ptrofs.zero) int_int_sg (Vint (Int.sub i (Int.repr 1)) :: nil) m).
+
+Inductive after_external: state -> reply li_c -> state -> Prop :=
+| after_external_intro
+    i ti m m' m'' m''' b_mem
+(*    (SUM: ti = sum (Int.sub i Int.one)) : *)
+    (FINDM: Genv.symbol_address ge _memoized Ptrofs.zero = Vptr b_mem Ptrofs.zero)
+    (STORE0: Mem.storev Mint32 m' (Vptr b_mem Ptrofs.zero) (Vint i) = Some m'')
+    (STORE0: Mem.storev Mint32 m'' (Vptr b_mem (Ptrofs.repr 4)) (Vint (Int.add ti i)) = Some m'''):
+    after_external (Interstate i m) (cr (Vint ti) m') (Returnstate (Int.add ti i) m''').
+
+Inductive step : state -> trace -> state -> Prop :=
+| step_zero
+    i m
+    (ZERO: i.(Int.intval) = 0%Z):
+    step (Callstate i m) E0 (Returnstate (Int.zero) m)
+| step_read
+    i b_mem m ti
+    (NZERO: i.(Int.intval) <> 0%Z)
+    (FINDM: Genv.symbol_address ge _memoized Ptrofs.zero= Vptr b_mem Ptrofs.zero)
+    (LOAD0: Mem.loadv Mint32 m (Vptr b_mem Ptrofs.zero) = Some (Vint i))
+    (LOAD1: Mem.loadv Mint32 m (Vptr b_mem (Ptrofs.repr 4)) = Some (Vint ti)):
+      step (Callstate i m) E0 (Returnstate ti m)
+| step_call
+    i m i' b_mem
+    (NZERO: i.(Int.intval) <> 0%Z)
+    (FINDM: Genv.symbol_address ge _memoized Ptrofs.zero = Vptr b_mem Ptrofs.zero)
+    (LOAD0: Mem.loadv Mint32 m (Vptr b_mem Ptrofs.zero) = Some (Vint i'))
+    (NEQ: i <> i'):
+    step (Callstate i m) E0 (Interstate i m).
+
+Inductive final_state: state -> reply li_c  -> Prop :=
+  | final_state_intro
+      s m :
+      final_state (Returnstate s m) (cr (Vint s) m).
+
+
+Definition valid_query (q : query li_c): bool := Genv.is_internal ge (cq_vf q).
 
 (*  match Genv.find_symbol se g_id with
     |Some b =>
@@ -96,6 +142,9 @@ Definition valid_query (q : query li_c): bool := true.
     |None => false
   end.*)
 
+End WITH_SE.
+*)
+(*
 Program Definition lts_Bspec :=
   {|
   Smallstep.step ge := step;
@@ -104,16 +153,27 @@ Program Definition lts_Bspec :=
   Smallstep.at_external := at_external;
   Smallstep.after_external := after_external;
   Smallstep.final_state := final_state;
-  globalenv := tt;
+  globalenv := Genv.globalenv se DemoB.prog;
   |}.
 
 End WITH_SE.
 
+*)
 Program Definition Bspec : Smallstep.semantics li_c li_c :=
   {|
-   Smallstep.skel := skel0;
+   Smallstep.skel := erase_program DemoB.prog;
    Smallstep.state := state;
-   Smallstep.activate := lts_Bspec
+   Smallstep.activate se :=
+     let ge := Genv.globalenv se DemoB.prog in
+     {|
+       Smallstep.step ge := step ge;
+       Smallstep.valid_query q := Genv.is_internal ge (cq_vf q);
+       Smallstep.initial_state := initial_state ge;
+       Smallstep.at_external := at_external ge;
+       Smallstep.after_external := after_external ge;
+       Smallstep.final_state := final_state;
+       globalenv := ge;
+     |}
    |}.
 
 
